src/Language/PlutusIR/Transform/DeadCode/Decide.v
@@ -21,10 +21,10 @@ Import ListNotations.
 
 Section Bindings.
 
-  Context (dec_Term : Term -> Term -> bool).
+  Context (dec_elim_Term : Term -> Term -> bool).
 
-  Definition dec_Binding (b b' : Binding) : bool := match b, b' with
-    | TermBind s vd t, TermBind s' vd' t' => Strictness_eqb s s' && VDecl_eqb vd vd' && dec_Term t t'
+  Definition dec_elim_Binding (b b' : Binding) : bool := match b, b' with
+    | TermBind s vd t, TermBind s' vd' t' => Strictness_eqb s s' && VDecl_eqb vd vd' && dec_elim_Term t t'
     | b, b' => Binding_eqb b b'
     end.
 
@@ -35,7 +35,7 @@ Section Bindings.
 
   Definition binding_was_there b' bs : bool :=
     match find (λ b, String.eqb (name_Binding b) (name_Binding b')) bs with
-      | Datatypes.Some b => dec_Binding b b'
+      | Datatypes.Some b => dec_elim_Binding b b'
       | None => false
     end
   .
@@ -45,7 +45,7 @@ Section Bindings.
   fix find (bs : list Binding) : bool :=
     match bs with
     | []      => false
-    | b :: bs => if String.eqb (name_Binding b) (name_Binding b') then dec_Binding b b' else find bs
+    | b :: bs => if String.eqb (name_Binding b) (name_Binding b') then dec_elim_Binding b b' else find bs
     end.
 
   (* This does not work in the termination checker, it doesn't see that b returned by find 
@@ -54,12 +54,12 @@ Section Bindings.
      what I did in the above definition*)
   Definition find_Binding' b' bs :=
     match find (λ b, String.eqb (name_Binding b) (name_Binding b')) bs with
-      | Datatypes.Some b => dec_Binding b b'
+      | Datatypes.Some b => dec_elim_Binding b b'
       | None => false
     end.
 
 
-  Definition dec_Bindings (bs bs' : list Binding) : bool :=
+  Definition dec_elim_Bindings (bs bs' : list Binding) : bool :=
     let bsn := map name_Binding bs in
     let bs'n := map name_Binding bs' in
     forallb (fun b => safely_removed b bs'n) bs &&
@@ -69,24 +69,24 @@ Section Bindings.
   (*
     forallb (fun b' =>
     match find (λ b, String.eqb (name_Binding b) (name_Binding b')) bs with
-      | Datatypes.Some b => dec_Binding b b'
+      | Datatypes.Some b => dec_elim_Binding b b'
       | None => false
     end
     ) bs'
    *)
 End Bindings.
 
-Fixpoint dec_Term (x y : Term) {struct x} : bool := match x, y with
+Fixpoint dec_elim_Term (x y : Term) {struct x} : bool := match x, y with
 
   | Let r bs t   , Let r' bs' t' => 
-      if dec_Bindings dec_Term bs bs'
+      if dec_elim_Bindings dec_elim_Term bs bs'
       then (* same let block, but bindings were removed *)
-        Recursivity_eqb r r' && dec_Term t t'
+        Recursivity_eqb r r' && dec_elim_Term t t'
       else (* t' is another let block, the whole block in the pre-term was removed *)
-        forallb (is_pure_binding []) bs && dec_Term t y (* Check whether the whole let was removed *)
+        forallb (is_pure_binding []) bs && dec_elim_Term t y (* Check whether the whole let was removed *)
   | Let _ bs t   , _ => 
-     forallb (is_pure_binding []) bs && dec_Term t y (* Check whether the whole let was removed *)
-  | _ , _ => is_cong dec_Term x y
+     forallb (is_pure_binding []) bs && dec_elim_Term t y (* Check whether the whole let was removed *)
+  | _ , _ => is_cong dec_elim_Term x y
 
   end
 .
